move encoding form tests into examples dir

src/Unicode/Utf16EncodingForm.dfy
@@ -138,33 +138,4 @@ module Utf16EncodingForm refines UnicodeEncodingForm {
     assert EncodeScalarValueDoubleWord(v) == m;
     v
   }
-
-  //
-  // Test lemmas
-  //
-
-  const TEST_SCALAR_VALUES: seq<(Unicode.ScalarValue, WellFormedCodeUnitSeq)> := [
-    // One code unit: dollar sign
-    (0x0024, [0x0024]),
-    // Two code units: money bag emoji
-    (0x1F4B0, [0xD83D, 0xDCB0])
-  ]
-
-  lemma TestEncodeScalarValue()
-    ensures forall pair | pair in TEST_SCALAR_VALUES
-      :: EncodeScalarValue(pair.0) == pair.1
-  {}
-
-  // Because surrogate code points are not Unicode scalar values, isolated UTF-16 code units in the range
-  // D800_16 .. DFFF_16 are ill-formed. (Section 3.9 D91)
-  const TEST_ILL_FORMED_SEQUENCES: seq<CodeUnitSeq> := [
-    [0xD800],
-    [0xDABC],
-    [0xDFFF]
-  ]
-
-  lemma TestDecodeIllFormedSequence()
-    ensures forall s | s in TEST_ILL_FORMED_SEQUENCES
-      :: DecodeCodeUnitSequenceChecked(s).None?
-  {}
 }
