src/Unicode/Utf8EncodingForm.dfy
@@ -254,37 +254,4 @@ module Utf8EncodingForm refines UnicodeEncodingForm {
     assert EncodeScalarValueQuadrupleByte(v) == m;
     v
   }
-
-  //
-  // Test lemmas
-  //
-
-  const TEST_SCALAR_VALUES: seq<(Unicode.ScalarValue, WellFormedCodeUnitSeq)> := [
-    // One byte: dollar sign
-    (0x0024, [0x24]),
-    // Two bytes: pound sign
-    (0x00A3, [0xC2, 0xA3]),
-    // Three bytes: euro sign
-    (0x20AC, [0xE2, 0x82, 0xAC]),
-    // Four bytes: money bag emoji
-    (0x1F4B0, [0xF0, 0x9F, 0x92, 0xB0])
-  ]
-
-  lemma TestEncodeScalarValue()
-    ensures forall pair | pair in TEST_SCALAR_VALUES
-      :: EncodeScalarValue(pair.0) == pair.1
-  {}
-
-  // Examples taken from description of Table 3-7.
-  const TEST_ILL_FORMED_SEQUENCES: seq<CodeUnitSeq> := [
-    // C0 is not well-formed as a first byte
-    [0xC0, 0xAF],
-    // 9F is not well-formed as a second byte when E0 is a well-formed first byte
-    [0xE0, 0x9F, 0x80]
-  ]
-
-  lemma TestDecodeIllFormedSequence()
-    ensures forall s | s in TEST_ILL_FORMED_SEQUENCES
-      :: DecodeCodeUnitSequenceChecked(s).None?
-  {}
 }
