examples/Unicode/Utf16EncodingFormExamples.dfy
@@ -1,0 +1,38 @@
+// RUN: %dafny /compile:0 "%s"
+
+/*******************************************************************************
+*  Copyright by the contributors to the Dafny Project
+*  SPDX-License-Identifier: MIT
+*******************************************************************************/
+
+include "../../src/Unicode/Utf16EncodingForm.dfy"
+
+module Utf16EncodingFormExamples {
+  import Unicode
+  import opened Utf16EncodingForm
+
+  const TEST_SCALAR_VALUES: seq<(Unicode.ScalarValue, WellFormedCodeUnitSeq)> := [
+    // One code unit: dollar sign
+    (0x0024, [0x0024]),
+    // Two code units: money bag emoji
+    (0x1F4B0, [0xD83D, 0xDCB0])
+  ]
+
+  lemma TestEncodeScalarValue()
+    ensures forall pair | pair in TEST_SCALAR_VALUES
+      :: EncodeScalarValue(pair.0) == pair.1
+  {}
+
+  // Because surrogate code points are not Unicode scalar values, isolated UTF-16 code units in the range
+  // D800_16 .. DFFF_16 are ill-formed. (Section 3.9 D91)
+  const TEST_ILL_FORMED_SEQUENCES: seq<CodeUnitSeq> := [
+    [0xD800],
+    [0xDABC],
+    [0xDFFF]
+  ]
+
+  lemma TestDecodeIllFormedSequence()
+    ensures forall s | s in TEST_ILL_FORMED_SEQUENCES
+      :: DecodeCodeUnitSequenceChecked(s).None?
+  {}
+}
